src/Examples/Interval/CallString/Call_String_Solver_Regression.thy
@@ -81,8 +81,8 @@ lemma nest_2_eqs_statement3:
                            (locals callee_state) (globs globals_state2)) Bot)))))]))"
   unfolding nest_2_eqs_def side_cfg_T_eff_keyed_seed_dg_def routed_extra_g_def
     routed_cmb_g_def routed_cmb_g_at_def
-  by (simp add: intra_predecessor_addr_list_def statement3_no_intra statement3_comb
-        statement3_targets statement3_no_calls nest_entry Let_def)
+  by (simp add: intra_predecessor_addr_list_def statement3_no_intra statement3_comb[simplified]
+        statement3_targets[simplified] statement3_no_calls nest_entry Let_def)
 
 lemma nest_1_eqs_statement3:
   "nest_1_eqs (Statement 3, ctx)
@@ -114,8 +114,8 @@ lemma nest_1_eqs_statement3:
                            (locals callee_state) (globs globals_state2)) Bot)))))]))"
   unfolding nest_1_eqs_def side_cfg_T_eff_keyed_seed_dg_def routed_extra_g_def
     routed_cmb_g_def routed_cmb_g_at_def
-  by (simp add: intra_predecessor_addr_list_def statement3_no_intra statement3_comb
-        statement3_targets statement3_no_calls nest_entry Let_def)
+  by (simp add: intra_predecessor_addr_list_def statement3_no_intra statement3_comb[simplified]
+        statement3_targets[simplified] statement3_no_calls nest_entry Let_def)
 
 end
 
